Manually commit some useful changes that happened during refactor on enter_smc_armdef

verified/entry.s.dfy
@@ -17,10 +17,30 @@ function l1pOfDispatcher(d:PageDb, p:PageNr) : PageNr
 predicate validERTransition(s:SysState, s':SysState)
 {
     reveal_validPageDb();
-    validSysState(s) && validSysState(s')
-    && s'.d == s.d && s'.hw.conf.ttbr0 == s.hw.conf.ttbr0 
-    && validL1PTPage(s.d, s.hw.conf.ttbr0)
-    && !hasStoppedAddrspace(s.d, s.hw.conf.ttbr0)
+    validSysState(s) && validSysState(s') &&
+    (var sd := s.g.g_cur_dispatcher;
+    var sd' := s'.g.g_cur_dispatcher;
+    validERTransitionHW(s.hw, s'.hw, s.d) &&
+    s.g.g_cur_dispatcher == s'.g.g_cur_dispatcher &&
+    validDispatcherPage(s.d, sd) && !hasStoppedAddrspace(s.d, sd) &&
+    validL1PTPage(s.d, l1pOfDispatcher(s.d, sd)) && 
+    validDispatcherPage(s'.d, sd') && !hasStoppedAddrspace(s'.d, sd) &&
+    validL1PTPage(s'.d, l1pOfDispatcher(s'.d, sd')) &&
+    l1pOfDispatcher(s.d, s.g.g_cur_dispatcher)  == s.hw.conf.ttbr0 &&
+    l1pOfDispatcher(s'.d, s'.g.g_cur_dispatcher) == s'.hw.conf.ttbr0)
+
+}
+
+predicate validERTransitionHW(hw:state, hw':state, d:PageDb)
+{
+    reveal_validPageDb();
+    reveal_ValidConfig();
+    ValidState(hw) && ValidState(hw')
+    && hw'.conf.ttbr0 == hw.conf.ttbr0 
+    && validL1PTPage(d, hw.conf.ttbr0)
+    && validL1PTPage(d, hw'.conf.ttbr0)
+    && !hasStoppedAddrspace(d, hw.conf.ttbr0)
+    && !hasStoppedAddrspace(d, hw'.conf.ttbr0)
 }
 
 predicate validEntryTransitionEnter(s:SysState,s':SysState,
@@ -31,23 +51,26 @@ predicate validEntryTransitionEnter(s:SysState,s':SysState,
     reveal_validPageDb();
     reveal_ValidConfig();
     reveal_ValidRegState();
-	var addrspace := s.d[s.d[dispPage].addrspace].entry;
+	//var addrspace := s.d[s.d[dispPage].addrspace].entry;
+    var l1p := l1pOfDispatcher(s.d, dispPage);
     
     validSysState(s') && s'.d == s.d &&
-    s'.hw.conf.ttbr0 == l1pOfDispatcher(s.d, dispPage) &&
+    s'.hw.conf.ttbr0 == l1p &&
     s'.hw.conf.cpsr.m  == User && s'.hw.conf.scr.ns == Secure &&
     
     s'.hw.regs[R0] == a1 && s'.hw.regs[R1] == a2 && s'.hw.regs[R2] == a3 &&
 
     s'.g.g_cur_dispatcher == dispPage &&
 
-    bankedRegsPreservedForMonitor(s, s') &&
-    WSMemInvariantExceptAddrspaceAtPage(s, s', l1pOfDispatcher(s.d, dispPage)) &&
+    bankedRegsPreservedForMonitor(s.hw, s'.hw) &&
+    WSMemInvariantExceptAddrspaceAtPage(s.hw, s'.hw, s.d, l1p) &&
 
-    sp_eval(Ins(MOVS_PCLR), s.hw, s'.hw, true) &&
+    // ENTER_ADDRSPACE is instruction evaluated on s->s'
+    // sp_eval(Ins(MOVS_PCLR), s.hw, s'.hw, true) &&
     OperandContents(s.hw, OLR) == s.d[dispPage].entry.entrypoint
 }
 
+/*
 predicate validEntryTransitionResume(s:SysState, s':SysState, dispPage:PageNr)
     requires validSysState(s)
     requires smc_resume(s.d, dispPage).1 == KEV_ERR_SUCCESS()
@@ -56,7 +79,7 @@ predicate validEntryTransitionResume(s:SysState, s':SysState, dispPage:PageNr)
     reveal_ValidConfig();
     var disp := s.d[dispPage].entry;
     
-    validSysState(s') && s'.d == s.d &&
+    validSysState(s') && // s'.d == s.d &&
     s'.hw.conf.ttbr0 == l1pOfDispatcher(s.d, dispPage) &&
     s'.hw.conf.cpsr.m  == User && s'.hw.conf.scr.ns == Secure &&
 
@@ -82,11 +105,12 @@ predicate validEntryTransitionResume(s:SysState, s':SysState, dispPage:PageNr)
     s'.hw.conf.cpsr == decode_psr(disp.ctxt.cpsr)) &&
     
     bankedRegsPreservedForMonitor(s, s') &&
-    WSMemInvariantExceptAddrspaceAtPage(s, s', l1pOfDispatcher(s.d, dispPage)) &&
+    WSMemInvariantExceptAddrspaceAtPage(s.hw, s'.hw, d, l1pOfDispatcher(s.d, dispPage)) &&
 
     sp_eval(Ins(MOVS_PCLR), s.hw, s'.hw, true) &&
     OperandContents(s.hw, OLR) == disp.ctxt.pc
 }
+*/
 
 predicate eqDisp(s:SysState, s':SysState) { s.g.g_cur_dispatcher == s'.g.g_cur_dispatcher }
 
@@ -94,19 +118,29 @@ predicate validEnter(s:SysState,s':SysState,
     dispPage:PageNr,a1:int,a2:int,a3:int)
     requires isUInt32(a1) && isUInt32(a2) && isUInt32(a3) && validSysState(s)
 {
-    // s1 (s)  : State on entry to the monitor
-    // s2      : State just before start of userspace execution.
-    // s3      : State between end of userspace execution and the exception handler
-    // s4      : State between the exception handler and re-entry to the monitor
-    // s5 (s') : State at the end of the monitor call
+    // s0 (s)  : State on entry to the monitor
+    // s1      : prior to MOVSPCLR that transitions to userspace/a
+    // s2      : post MOVS State just before start of userspace execution.
+    // s3      : Exceptional where handler must be called
+    // s4      : State at start of exception handler
+    // s5      : State at start of transition back to smc_handler
+    // s6      : State on re-entry to smc_handler
+    // s7 (s') : State at the end of the monitor call/
+    //
+    // s3 == s4 except not in exceptional state in s4
+    // s5 == s6 except branch has happened
     
     smc_enter(s.d, dispPage, a1, a2, a3).1 != KEV_ERR_SUCCESS() ||
-    (exists s2, s3, s4 :: validEntryTransitionEnter(s,s2,dispPage,a1,a2,a3)
-        && userspaceExecution(s2, s3)
-        && exception(s3, s4)
-        && monitorReturn(s4, s'))
+    (exists s2, s3, s4, s5 :: validSysState(s2) && validSysState(s3)
+        && validSysState(s4) && validSysState(s5)
+        && validEntryTransitionEnter(s,s2,dispPage,a1,a2,a3)
+        && s3.d == s2.d && userspaceExecution(s2.hw, s3.hw, s2.d)
+        && s4.d == s3.d && handlerCalled(s3.hw, s4.hw)
+        && exceptionHandled(s4, s5)
+        && monitorReturn(s5, s'))
 }
 
+/*
 predicate validResume(s:SysState,s':SysState,dispPage:PageNr)
     requires validSysState(s)
 {
@@ -119,22 +153,33 @@ predicate validResume(s:SysState,s':SysState,dispPage:PageNr)
     smc_resume(s.d, dispPage).1 != KEV_ERR_SUCCESS() ||
     (exists s2, s3, s4 :: validEntryTransitionResume(s,s2,dispPage) 
         && userspaceExecution(s2, s3)
-        && exception(s3, s4)
+        && exceptionHandled(s3, s4)
         && monitorReturn(s4, s'))
+}
+*/
+
+predicate exceptionHandled(s:SysState,s':SysState)
+    ensures exceptionHandled(s, s') ==> 
+        validERTransition(s, s') &&
+        WSMemInvariantExceptAddrspace(s.hw, s'.hw, s.d)
+{
+    svc(s,s') || irqfiq(s,s') || abort(s,s')
+}
+
+predicate handlerCalled(hw:state,hw':state)
+{
+    !hw.conf.ex.none? &&
+    ValidState(hw) &&
+    hw'  == hw.(conf := hw.conf.(ex := none))
 }
 
 predicate monitorReturn(s:SysState,s':SysState)
 {
     reveal_ValidRegState();
     validERTransition(s, s')
-    && (var ret := s'.hw.regs[R0];
-        var dispPage := s.g.g_cur_dispatcher;
-        if(ret == KEV_ERR_INTERRUPTED() || ret == KEV_ERR_FAULT()) then
-            s'.d[dispPage].entry.entered == true 
-        else // SUCCESS
-            s'.d[dispPage].entry.entered == false)
-    && WSMemInvariantExceptAddrspace(s, s')
-    && bankedRegsPreservedForMonitor(s, s')
+    && s'.d == s.d
+    && WSMemInvariantExceptAddrspace(s.hw, s'.hw, s.d)
+    && bankedRegsPreservedForMonitor(s.hw, s'.hw)
     && s'.hw.conf.scr.ns == NotSecure
 }
 
@@ -145,15 +190,14 @@ predicate svc(s:SysState,s':SysState)
     validERTransition(s, s') &&
     s.hw.conf.cpsr.m == Supervisor &&
     s'.hw.conf.cpsr.m == Monitor &&
+    s.hw.conf.ex.svc? &&
     
-    WSMemInvariantExceptAddrspace(s, s') &&
-    bankedRegsPreservedForMonitor(s, s') &&
+    WSMemInvariantExceptAddrspace(s.hw, s'.hw, s.d) &&
+    bankedRegsPreservedForMonitor(s.hw, s'.hw) &&
     
     s'.hw.regs[R0] == KEV_ERR_SUCCESS()  &&
         
-    (var dispPage := s.g.g_cur_dispatcher;
-    validDispatcherPage(s'.d, dispPage) &&
-    s'.d[dispPage].addrspace == s.d[dispPage].addrspace)
+    s'.d == s.d
 }
 
 predicate irqfiq(s:SysState,s':SysState)
@@ -165,10 +209,10 @@ predicate irqfiq(s:SysState,s':SysState)
     validERTransition(s, s') &&
     s.hw.conf.cpsr.m == Monitor &&
     s'.hw.conf.cpsr.m == Monitor &&
+    (s.hw.conf.ex.irq? || s.hw.conf.ex.fiq?) &&
 
-    s.d == s'.d &&
-    WSMemInvariantExceptAddrspace(s, s') &&
-    bankedRegsPreservedForMonitor(s, s') &&
+    WSMemInvariantExceptAddrspace(s.hw, s'.hw, s.d) &&
+    bankedRegsPreservedForMonitor(s.hw, s'.hw) &&
     
     // Interrupts can be taken from other modes, but the interrupt should
     // only re-enter monitor mode when taken from user mode. The following 
@@ -183,7 +227,8 @@ predicate irqfiq(s:SysState,s':SysState)
     s'.d[dispPage].entry.entered == true &&
     s'.d[dispPage].entry.ctxt.regs == s.hw.regs &&
     s'.d[dispPage].entry.ctxt.pc == OperandContents(s.hw, OLR) &&
-    s'.d[dispPage].entry.ctxt.cpsr == s.hw.sregs[cpsr])
+    s'.d[dispPage].entry.ctxt.cpsr == s.hw.sregs[cpsr] &&
+    equivalentExceptPage(s.d, s'.d, dispPage))
 
 }
 
@@ -194,10 +239,11 @@ predicate abort(s:SysState,s':SysState)
     validERTransition(s, s') &&
     s.hw.conf.cpsr.m == Abort  &&
     s'.hw.conf.cpsr.m == Monitor &&
+    s.hw.conf.ex.abt? &&
     
     s.d == s'.d &&
-    bankedRegsPreservedForMonitor(s, s') &&
-    WSMemInvariantExceptAddrspace(s, s') &&
+    bankedRegsPreservedForMonitor(s.hw, s'.hw) &&
+    WSMemInvariantExceptAddrspace(s.hw, s'.hw, s.d) &&
 
     s'.hw.regs[R0] == KEV_ERR_FAULT() &&
     
@@ -211,55 +257,49 @@ predicate abort(s:SysState,s':SysState)
 // Userspace Execution
 //-----------------------------------------------------------------------------
 
-//The code executing in userspace is possibly malicious. This models its limitations.
-predicate userspaceExecution(s:SysState, s':SysState)
+predicate userspaceExecution(hw:state, hw':state, d:PageDb)
 {
-    validERTransition(s, s')
-    && s.hw.conf.cpsr.m == User && s.hw.conf.cpsr.m == User
-    && WSMemInvariantExceptAddrspace(s, s')
-    && bankedRegsPreservedForMonitor(s, s')
+    validERTransitionHW(hw, hw', d)
+    && hw.conf.cpsr.m == User && hw'.conf.cpsr.m == User
+    && WSMemInvariantExceptAddrspace(hw, hw', d)
+    && bankedRegsPreservedForMonitor(hw, hw')
+    && !hw'.conf.ex.none?
 }
 
-predicate exception(s:SysState, s':SysState)
-    ensures exception(s, s') ==> 
-        validERTransition(s, s') &&
-        WSMemInvariantExceptAddrspace(s, s')
-{
-    svc(s,s') || irqfiq(s,s') || abort(s,s')
-}
-
-// All writeable and secure memory addresses except the ones in the active l1
-// page table have their contents preserved
-
-predicate WSMemInvariantExceptAddrspace(s:SysState, s':SysState)
-    requires validERTransition(s, s')
-    //requires userEnteredState(s) && userEnteredState(s') && s'.d == s.d
-{
-    WSMemInvariantExceptAddrspaceAtPage(s, s', s.hw.conf.ttbr0)
-}
-
-predicate WSMemInvariantExceptAddrspaceAtPage(s:SysState, s':SysState, l1p:PageNr)
-    requires validSysState(s) && validSysState(s') && s.d == s'.d
-    requires validL1PTPage(s.d, l1p)
-    requires (validPageDbImpliesWellFormed(s.d); !hasStoppedAddrspace(s.d, l1p))
-{
-    ValidState(s'.hw) && AlwaysInvariant(s.hw, s'.hw) &&
-    s.hw.m.globals == s'.hw.m.globals &&
-    forall i :: i in s.hw.m.addresses && address_is_secure(i) &&
-        !memSWrInAddrspace(s.d, l1p, i) ==>
-            s.hw.m.addresses[i] == s'.hw.m.addresses[i]
-}
-
-predicate bankedRegsPreservedForMonitor(s:SysState, s':SysState)
+predicate bankedRegsPreservedForMonitor(hw:state, hw':state)
+    requires ValidState(hw) && ValidState(hw')
 {
         reveal_ValidRegState();
         reveal_ValidConfig();
         var m := Monitor;
-        validSysState(s) && validSysState(s') &&
-        s.hw.conf.spsr[m] == s'.hw.conf.spsr[m] &&
-        s.hw.regs[LR(m)] == s'.hw.regs[LR(m)] &&
-        s.hw.regs[SP(m)] == s'.hw.regs[SP(m)]
+        hw.conf.spsr[m] == hw'.conf.spsr[m] &&
+        hw.regs[LR(m)] == hw'.regs[LR(m)] &&
+        hw.regs[SP(m)] == hw'.regs[SP(m)]
 }
+
+// All writeable and secure memory addresses except the ones in the active l1
+// page table have their contents preserved
+predicate WSMemInvariantExceptAddrspace(hw:state, hw':state, d:PageDb)
+    // requires validERTransition(s, s')
+    // requires userEnteredState(s) && userEnteredState(s')
+    requires validERTransitionHW(hw, hw', d)
+{
+    WSMemInvariantExceptAddrspaceAtPage(hw, hw', d, hw.conf.ttbr0)
+}
+
+predicate WSMemInvariantExceptAddrspaceAtPage(hw:state, hw':state, 
+        d:PageDb, l1p:PageNr)
+    requires ValidState(hw) && ValidState(hw')
+    requires validL1PTPage(d, l1p)
+    requires (validPageDbImpliesWellFormed(d); !hasStoppedAddrspace(d, l1p))
+{
+    (forall m:mem :: m in hw.m.addresses <==> m in hw'.m.addresses) &&
+    hw.m.globals == hw'.m.globals &&
+    forall i :: i in hw.m.addresses && address_is_secure(i) &&
+        !memSWrInAddrspace(d, l1p, i) ==>
+            hw.m.addresses[i] == hw'.m.addresses[i]
+}
+
 
 // Is the page secure, writeable, and in the L1PT
 predicate pageSWrInAddrspace(d:PageDb, l1p:PageNr, p:PageNr)
@@ -287,6 +327,18 @@ predicate pageSWrInL2PT(l2pt:seq<L2PTE>, p:PageNr)
         case NoMapping => false
         case SecureMapping(p', w, e) => w && p' == p
         case InsecureMapping(p',w) => false)
+}
+
+
+
+// A purely abstract version of the memory invariant
+predicate equivalentExceptPage(d:PageDb, d':PageDb, p:PageNr)
+    requires validPageNr(p)
+    requires validPageDb(d) && validPageDb(d')
+{
+    validPageDbImpliesWellFormed(d);
+    validPageDbImpliesWellFormed(d');
+    forall p' :: validPageNr(p') && p' != p ==> d[p'] == d'[p]
 }
 
 
